@prefix serviceType: <https://purl.org/ctdl/vocabs/agentServiceType/> .
@prefix dc: <http://purl.org/dc/elements/1.1/> .
@prefix dct: <http://purl.org/dc/terms/> .
@prefix skos: <http://www.w3.org/2004/02/skos/core#> .
@prefix schema: <http://schema.org/> .
@prefix rdf: <http://www.w3.org/1999/02/22-rdf-syntax-ns#> .
@prefix rdfs: <http://www.w3.org/2000/01/rdf-schema#> .
@prefix xsd: <http://www.w3.org/2001/XMLSchema#> .
@prefix adms: <http://www.w3.org/ns/adms#> .
@prefix bibo: <http://purl.org/ontology/bibo/status/> .
@prefix vs: <http://www.w3.org/2003/06/sw-vocab-status/ns#> .

# AGENT SERVICE TYPE VOCABULARY DESCRIPTION
serviceType: a skos:ConceptScheme;
    dc:title "CTI Cost Type Vocabulary" ;
    dc:creator "Credential Transparency Initiative (CTI)"@en-US ;
    dc:description "A concept scheme that defines agent service types."@en-US ;
    dct:created "2016-09-08"^^xsd:date ;
    dct:license <http://creativecommons.org/licenses/by/4.0/> ;                         
    adms:status bibo:draft . 
   
# CONCEPT: ACCREDIT SERVICE
serviceType:AccreditService a skos:Concept;
    skos:prefLabel "Accredit Service"@en-US; 
    skos:definition "The services provided by an organization that has been given the authority by a private, professional or governmental agency to conduct formal assessments, (often a document review and on-site visit), of a credential issuing organization to determine if it meets a specified set of standards or criteria."@en-US;
    skos:inScheme serviceType: ;
    vs:term_status "unstable" .
       
# CONCEPT: APPROVE SERVICE
serviceType:ApproveService a skos:Concept;
    skos:prefLabel "Approve Service"@en-US; 
    skos:definition "The services provided by a private or governmental body that reviews a credential issuing organization against some criteria for recognition."@en-US;
    skos:inScheme serviceType: ;
    vs:term_status "unstable" .
       
# CONCEPT: CONFER SERVICE
serviceType:ConferService a skos:Concept;
    skos:prefLabel "Confer Service"@en-US; 
    skos:definition "The services provided by an organization that grants credential."@en-US;
    skos:inScheme serviceType: ;
    vs:term_status "unstable" .
       
# CONCEPT: ENDORSE SERVICE
serviceType:EndorseService a skos:Concept;
    skos:prefLabel "Endorse Service"@en-US; 
    skos:definition "The services provided by a private organization that public declares some level of quality of the services and may or may not be based on some type of criteria."@en-US;
    skos:inScheme serviceType: ;
    vs:term_status "unstable" .
       
# CONCEPT: MONITOR SERVICE
serviceType:MonitorService a skos:Concept;
    skos:prefLabel "Monitor Service"@en-US; 
    skos:definition "The services provided by an organization that include observation, checking, reporting of data, or keeping systemic records of a process, activity, or quality of a activity."@en-US;
    skos:inScheme serviceType: ;
    vs:term_status "unstable" .
       
# CONCEPT: OFFER CREDENTIAL SERVICE
serviceType:OfferCredentialService a skos:Concept;
    skos:prefLabel "Offer Credential Service"@en-US; 
    skos:definition "The services provided by an organization that creates and awards a credential."@en-US;
    skos:inScheme serviceType: ;
    vs:term_status "unstable" .
       
# CONCEPT: RECOGNIZE SERVICE
serviceType:RecognizeService a skos:Concept;
    skos:prefLabel "Recognize Service"@en-US; 
    skos:definition "The services provided by an organization that   acknowledges another entity that may or may not have met some criteria."@en-US;
    skos:inScheme serviceType: ;
    vs:term_status "unstable" .
       
# CONCEPT: REGULATE SERVICE
serviceType:RegulateService a skos:Concept;
    skos:prefLabel "Regulate Service"@en-US; 
    skos:definition "The services provided by a governmental agency that issues a credential and is legal enforceable."@en-US;
    skos:inScheme serviceType: ;
    vs:term_status "unstable" .
       
# CONCEPT: RENEW SERVICE
serviceType:RenewService a skos:Concept;
    skos:prefLabel "Renew Credential Service"@en-US; 
    skos:definition "The services provided by an organization include renewal of an awarded credential."@en-US;
    skos:inScheme serviceType: ;
    vs:term_status "unstable" .
       
# CONCEPT: REVOCATION SERVICE
serviceType:RevokeService a skos:Concept;
    skos:prefLabel "Revoke Credential Service"@en-US; 
    skos:definition "Due process procedures created by an organization to removal a credential from the holder."@en-US;
    skos:inScheme serviceType: ;
    vs:term_status "unstable" .
       
# CONCEPT: UPDATE CREDENTIAL VERSION SERVICE
serviceType:UpdateVersionService a skos:Concept;
    skos:prefLabel "Update Credential Version Service"@en-US; 
    skos:definition "The services provided by an organization includes updating of a credential."@en-US;
    skos:inScheme serviceType: ;
    vs:term_status "unstable" .
       
# CONCEPT: VALIDATE SERVICE
serviceType:ValidateService a skos:Concept;
    skos:prefLabel "Validate Service"@en-US; 
    skos:definition "Develops scientific general accepted procedures to validate the content that supports the credential."@en-US;
    skos:inScheme serviceType: ;
    vs:term_status "unstable" .
       
# CONCEPT: VERIFY SERVICE
serviceType:VerifyService a skos:Concept;
    skos:prefLabel "Verify Holder Service"@en-US; 
    skos:definition "The services provided by an organization to verify to another person, organization or governmental agency that the credential is held by the holder."@en-US;
    skos:inScheme serviceType: ;
    vs:term_status "unstable" .
       
# CONCEPT: QUALITY ASSURANCE SERVICE
serviceType:QualityAssuranceService a skos:Concept;
    skos:prefLabel "Quality Assurance Service"@en-US; 
    skos:definition "The services provided by an organization that makes a judgment about the quality of service based on requirements, criteria and/or standards."@en-US;
    skos:inScheme serviceType: ;
    vs:term_status "unstable" .
       
# CONCEPT: CONTINUOUS IMPROVEMENT SERVICE
serviceType:ContinuousImprovementService a skos:Concept;
    skos:prefLabel "Continuous Quality Improvement Service"@en-US; 
    skos:definition "The services provided by an organization include assessing the presence and success of processes for creating an environment in which management and workers strive to constantly improve quality."@en-US;
    skos:inScheme serviceType: ;
    vs:term_status "unstable" .
       
# CONCEPT: CONFORMANCE ASSESSMENT SERVICE
serviceType:ConformanceAssessmentService a skos:Concept;
    skos:prefLabel "Conformance Assessment Service"@en-US; 
    skos:definition "The services provided by an organization include activities to determine, directly or indirectly, that a resource meets relevant standards and fulfills relevant requirements."@en-US;
    skos:inScheme serviceType: ;
    vs:term_status "unstable" .
       
# CONCEPT: COMPLIANCE SERVICE
serviceType:ComplianceService a skos:Concept;
    skos:prefLabel "Compliance Service"@en-US; 
    skos:definition "Generally governmental services provided by an authoritative agent that determines conformance to fulfilling official requirements."@en-US;
    skos:inScheme serviceType: ;
    vs:term_status "unstable" .