@prefix qaPurpose: <https://purl.org/ctdl/vocabs/agentQAPurpose/> .
@prefix dc: <http://purl.org/dc/elements/1.1/> .
@prefix dct: <http://purl.org/dc/terms/> .
@prefix skos: <http://www.w3.org/2004/02/skos/core#> .
@prefix schema: <http://schema.org/> .
@prefix rdf: <http://www.w3.org/1999/02/22-rdf-syntax-ns#> .
@prefix rdfs: <http://www.w3.org/2000/01/rdf-schema#> .
@prefix xsd: <http://www.w3.org/2001/XMLSchema#> .
@prefix adms: <http://www.w3.org/ns/adms#> .
@prefix bibo: <http://purl.org/ontology/bibo/status/> .
@prefix vs: <http://www.w3.org/2003/06/sw-vocab-status/ns#> .

# AGENT QUALITY ASSURANCE PURPOSE VOCABULARY DESCRIPTION
qaPurpose: a skos:ConceptScheme;
    dc:title "CTI Agent Quality Assurance Purpose Vocabulary" ;
    dc:creator "Credential Transparency Initiative (CTI)"@en-US ;
    dc:description "A concept scheme that defines the purposes of QA agents."@en-US ;
    dct:created "2016-09-07"^^xsd:date ;
    dct:license <http://creativecommons.org/licenses/by/4.0/> ;                         
    adms:status bibo:draft . 
   
# CONCEPT: GOVERNMENT REQUIREMENTS
qaPurpose:GovernmentRequirements a skos:Concept;
    skos:prefLabel "Government Requirements"@en-US; 
    skos:definition "The main purpose of the agent's quality assurance is to meet government requirements."@en-US;
    skos:inScheme qaPurpose: ;
    vs:term_status "unstable" .
       
# CONCEPT: ENTRY TO PRACTICE
qaPurpose:EntryToPractice a skos:Concept;
    skos:prefLabel "Entry to Practice"@en-US; 
    skos:definition "The main purpose of the agent's quality assurance is to provide entry into practice."@en-US;
    skos:inScheme qaPurpose: ;
    vs:term_status "unstable" .
       
# CONCEPT: FEDERAL FINANCIAL AID
qaPurpose:FederalFinancialAid a skos:Concept;
    skos:prefLabel "Enables Federal Financial Aid"@en-US; 
    skos:definition "The main purpose of the agent's quality assurance is to enable federal financial aid."@en-US;
    skos:inScheme qaPurpose: ;
    vs:term_status "unstable" .
       
# CONCEPT: STATE FINANCIAL AID
qaPurpose:StateFinancialAid a skos:Concept;
    skos:prefLabel "Enables State Financial Aid"@en-US; 
    skos:definition "The main purpose of the agent's quality assurance is to enable state financial aid."@en-US;
    skos:inScheme qaPurpose: ;
    vs:term_status "unstable" .
       
# CONCEPT: EMPLOYER TYUITIONL AID
qaPurpose:EmployerTuitionAid a skos:Concept;
    skos:prefLabel "Enables Employer Tuition Aid"@en-US; 
    skos:definition "The main purpose of the agent's quality assurance is to enable employer tuition aid."@en-US;
    skos:inScheme qaPurpose: ;
    vs:term_status "unstable" .
       
# CONCEPT: UNACCREDITED PROGRAM FOUNDATION AID
qaPurpose:UnaccreditedProgramFoundationAid a skos:Concept;
    skos:prefLabel "Enables Unaccredited Program Foundation Aid"@en-US; 
    skos:definition "The main purpose of the agent's quality assurance is to enable unaccredited program foundation aid."@en-US;
    skos:inScheme qaPurpose: ;
    vs:term_status "unstable" .
       
# CONCEPT: ASSIST EMPLOYERS
qaPurpose:AssistEmployers a skos:Concept;
    skos:prefLabel "Assists Employers Seeking Competent Practitioners"@en-US; 
    skos:definition "The main purpose of the agent's quality assurance is to assist employers seeking competent practitioners."@en-US;
    skos:inScheme qaPurpose: ;
    vs:term_status "unstable" .
       
# CONCEPT: PROMOTE CAREER MOBILITY
qaPurpose:PromoteCareerMobility a skos:Concept;
    skos:prefLabel "Promotes Professional Advancement and Career Mobility"@en-US; 
    skos:definition "Assists Employers Seeking Competent Practitioners"@en-US;
    skos:inScheme qaPurpose: ;
    vs:term_status "unstable" .
       
# CONCEPT: FULFILLS ELIGIBILITY REQUIREMENTS
qaPurpose:FulfillsEligibilityRequirements a skos:Concept;
    skos:prefLabel "Fulfills Eligibility Requirements"@en-US; 
    skos:definition "The main purpose of the agent's quality assurance is to fulfill eligibility requirements."@en-US;
    skos:inScheme qaPurpose: ;
    vs:term_status "unstable" .