@prefix assessMethod: <https://purl.org/ctdl/vocabs/assessmentMethod/> .
@prefix dc: <http://purl.org/dc/elements/1.1/> .
@prefix dct: <http://purl.org/dc/terms/> .
@prefix skos: <http://www.w3.org/2004/02/skos/core#> .
@prefix schema: <http://schema.org/> .
@prefix rdf: <http://www.w3.org/1999/02/22-rdf-syntax-ns#> .
@prefix rdfs: <http://www.w3.org/2000/01/rdf-schema#> .
@prefix xsd: <http://www.w3.org/2001/XMLSchema#> .
@prefix adms: <http://www.w3.org/ns/adms#> .
@prefix bibo: <http://purl.org/ontology/bibo/status/> .
@prefix vs: <http://www.w3.org/2003/06/sw-vocab-status/ns#> .

# ASSESSMENT METHOD VOCABULARY DESCRIPTION
assessMethod: a skos:ConceptScheme;
    dc:title "CTI Assessment Method Vocabulary" ;
    dc:creator "Credential Transparency Initiative (CTI)"@en-US ;
    dc:description "A concept scheme that defines methods of assessment."@en-US ;
    dct:created "2016-09-07"^^xsd:date ;
    dct:source "Sources consulted include Integrated Postsecondary Education Data System (IPEDS)."@en-US ;
    dct:license <http://creativecommons.org/licenses/by/4.0/> ;                         
    adms:status bibo:draft . 
   
# CONCEPT: ACHIEVEMENT TEST
assessMethod:AchievementTest a skos:Concept;
    skos:prefLabel "Achievement Test"@en-US; 
    skos:definition "A frequently  standardized test developed to measure skills and knowledge learned in a given educational level."@en-US;
    skos:inScheme assessMethod: ;
    vs:term_status "unstable" .
  
# CONCEPT: ADVANCED PLACEMENT TEST
assessMethod:AdvancedPlacementTest a skos:Concept ;
    skos:prefLabel "Advanced Placement Test"@en-US ; 
    skos:definition "Assessment based on scores from examination at the conclusion of advanced placement courses in secondary school for purposes including postsecondary-level credit or placement in advanced postseconday-level courses."@en-US ;
    skos:inScheme assessMethod: ;
    vs:term_status "unstable" . 
  
# CONCEPT: ALTERNATE ASSESSMENT
assessMethod:AlternateAssessment a skos:Concept ;
    skos:prefLabel "Alternate Assessment"@en-US ;
    skos:definition "Assessments other than traditional paper-and-pencil, short answer tests that focus on what students can do without emphasizing their weaknesses, especially in test-taking skills."@en-US ;
    dct:source "Adapted from: http://www.learnnc.org/lp/pages/7041"@en-US ;
    skos:inScheme assessMethod: ;
    vs:term_status "unstable" . 
  
# CONCEPT: CAPSTONE PROJECT
assessMethod:CapstoneProject a skos:Concept ;
    skos:prefLabel "Capstone/Exhibition Project"@en-US ;
    skos:definition "A multifaceted assignment that serves as a culminating academic and intellectual experience for students, typically during their final year of study."@en-US ;
    dct:source "Adapted from: http://edglossary.org/capstone-project/"@en-US ;
    skos:inScheme assessMethod: ;
    vs:term_status "unstable" . 
    
# CONCEPT: CLASS PARTICIPATION
assessMethod:ClassParticipation a skos:Concept ;
    skos:prefLabel "Class Participation"@en-US ;
    skos:definition "Assessment based on the extent and quality of contributions to discussion."@en-US ;
    skos:inScheme assessMethod: ;
    vs:term_status "unstable" .  
    
# CONCEPT: DEMONSTRATION
assessMethod:Demonstration a skos:Concept ;
    skos:prefLabel "Demonstration"@en-US ;
    skos:definition "Written record of an observed demonstration including explanation of factors assessed."@en-US ;
    skos:inScheme assessMethod: ;
    vs:term_status "unstable" .
    
# CONCEPT: ESSAY
assessMethod:Essay a skos:Concept ;
    skos:prefLabel "Essay"@en-US ;
    skos:definition "Short piece of writing that fashions a coherent set of ideas on a particular subject."@en-US ;
    skos:inScheme assessMethod: ;
    vs:term_status "unstable" .             
     
# CONCEPT: JOB EVALUATION
assessMethod:JobEvaluation a skos:Concept ;
    skos:prefLabel "Job Evaluation"@en-US ;
    skos:definition "Supervisor's evaluation of on-the-job performance."@en-US ;
    skos:inScheme assessMethod: ;
    vs:term_status "unstable" .
    
# CONCEPT: MULTIPLE CHOICE TEST
assessMethod:MultipleChoiceTest a skos:Concept ;
    skos:prefLabel "Multiple Choice Test"@en-US ;
    skos:definition "Test comprised of questions accompanied by several possible answers from which the candidate must try to choose the correct one."@en-US ;
    skos:inScheme assessMethod: ;
    vs:term_status "unstable" . 
    
# CONCEPT: OBSERVATION
assessMethod:Observation a skos:Concept ;
    skos:prefLabel "Observation"@en-US ;
    skos:definition "Evaluation based on expert observation of performace of a prescribed action."@en-US ;
    skos:inScheme assessMethod: ;
    vs:term_status "unstable" .
    
# CONCEPT: ORAL EXAMINATION
assessMethod:OralExam a skos:Concept ;
    skos:prefLabel "Oral Examination"@en-US ;
    skos:definition "Evaluation based on oral responses to questions."@en-US ;
    skos:inScheme assessMethod: ;
    vs:term_status "unstable" .  
    
# CONCEPT: PORTFOLIO
assessMethod:Portfolio a skos:Concept ;
    skos:prefLabel "Portfolio"@en-US ;
    skos:definition "Evaluation based on the assessment of creator-selected artifacts demonstrating the knowledge or skills of their creator."@en-US ;
    skos:inScheme assessMethod: ;
    vs:term_status "unstable" .
    
# CONCEPT: RELATED PERFORMANCE
assessMethod:RelatedPerformance a skos:Concept ;
    skos:prefLabel "Related Performance"@en-US ;
    skos:definition "[ TBD ]"@en-US ;
    skos:inScheme assessMethod: ;
    vs:term_status "unstable" . 
    
# CONCEPT: SHORT ANSWER EXAMINATION
assessMethod:ShortAnswer a skos:Concept ;
    skos:prefLabel "Short Answer Examination"@en-US ;
    skos:definition "Short-answer evaluation usually testing whether a person has a factual understanding of the relevant information."@en-US ;
    skos:inScheme assessMethod: ;
    vs:term_status "unstable" .                         