@prefix credType: <https://w3id.org/ctdl/vocabs/credentialType/> .
@prefix dc: <http://purl.org/dc/elements/1.1/> .
@prefix dct: <http://purl.org/dc/terms/> .
@prefix skos: <http://www.w3.org/2004/02/skos/core#> .
@prefix schema: <http://schema.org/> .
@prefix rdf: <http://www.w3.org/1999/02/22-rdf-syntax-ns#> .
@prefix rdfs: <http://www.w3.org/2000/01/rdf-schema#> .
@prefix xsd: <http://www.w3.org/2001/XMLSchema#> .
@prefix adms: <http://www.w3.org/ns/adms#> .
@prefix bibo: <http://purl.org/ontology/bibo/status/> .
@prefix vs: <http://www.w3.org/2003/06/sw-vocab-status/ns#> .

credType: a skos:ConceptScheme;
   dc:title "CTI Credential Type Vocabulary" ;
   dc:creator "Credential Transparency Initiative (CTI)"@en-US ;
   dc:description "A concept scheme that defines the categories of credentials in the credential ecosystem."@en-US ;
   dct:created "2016-05-04"^^xsd:date ;
   dct:license <http://creativecommons.org/licenses/by/4.0/> ;
   skos:hasTopConcept credType:apprenticeship;
   skos:hasTopConcept credType:certificate;
   skos:hasTopConcept credType:certification;
   skos:hasTopConcept credType:degree;
   skos:hasTopConcept credType:digitalBadge;
   skos:hasTopConcept credType:diploma;
   skos:hasTopConcept credType:license;
   skos:hasTopConcept credType:microCredential;
   skos:hasTopConcept credType:militaryCredential;
   skos:hasTopConcept credType:nanodegree;                          
   adms:status bibo:draft .  

# APPRENTICESHIP  
credType:apprenticeship a skos:Concept;
   skos:prefLabel "Apprenticeship"@en-US; 
   skos:definition "Skill-based occupational proficiency determined by trade organizations."@en-US;
   skos:inScheme credType: ;
   vs:term_status "unstable" .

# CERTIFICATE    
credType:certificate a skos:Concept;
  skos:prefLabel "Certificate"@en-US; 
  skos:definition "Document (letter, card, or other medium) awarded to certificate holders that designates the successful completion of a certificate program’s requisites."@en-US;
  skos:narrower credType:jobSkillsCertificate ;
  skos:narrower credType:industryJobCertificate ;
  skos:inScheme credType: ;
  vs:term_status "unstable" .

# JOB SKILLS CERTIFICATE  
credType:jobSkillsCertificate a skos:Concept;
  skos:prefLabel "Certificate (Job Skills)"@en-US; 
  skos:definition "Document (letter, card, or other medium) awarded to certificate holders that designates the successful completion of a certificate program’s requisites for a specific job skill."@en-US;
  skos:broader credType:certificate;
  skos:inScheme credType: ;
  vs:term_status "unstable" .
  
# INDUSTRY JOB  CERTIFICATE  
credType:industryJobCertificate a skos:Concept;
  skos:prefLabel "Certificate (Industry Job)"@en-US; 
  skos:definition "Document (letter, card, or other medium) awarded to certificate holders that designates the successful completion of a certificate program’s requisites for a specific industry job."@en-US;
  skos:broader credType:certificate;
  skos:inScheme credType: ;
  vs:term_status "unstable" .
  
# CERTIFICATION    
credType:certification a skos:Concept;
  skos:prefLabel "Certification"@en-US; 
  skos:definition "Designation earned by a person to assure qualification to perform a job or task through assessment and issuance of a renewable certification."@en-US;
  skos:inScheme credType: ;
  vs:term_status "unstable" . 
  
# DEGREE    
credType:degree a skos:Concept ;
  skos:prefLabel "Degree"@en-US ; 
  skos:definition "State of recognized completion of studies that is earned or conferred at an accredited school or postsecondary institution."@en-US ;
  skos:narrower credType:associateDegree ; 
  skos:narrower credType:bachelorDegree ;
  skos:narrower credType:graduateDegree ; 
  skos:narrower credType:doctoralDegree ;    
  skos:inScheme credType: ;
  vs:term_status "unstable" .
  
# ASSOCIATE DEGREE
credType:associateDegree a skos:Concept ;
  skos:prefLabel "Associate Degree"@en-US ; 
  skos:definition "Undergraduate academic degree awarded in the U.S. by colleges and universities upon completion of a course of study lasting two years."@en-US ;
  skos:broader credType:degree ;
  skos:inScheme credType: ;
  vs:term_status "unstable" .
  
# BACHELOR DEGREE
credType:bachelorDegree a skos:Concept ;
  skos:prefLabel "Bachelor Degree"@en-US ; 
  skos:definition "A bachelor degree is usually earned for an undergraduate course of study that normally requires four years of study."@en-US ;
  skos:broader credType:degree ;
  skos:inScheme credType: ;
  vs:term_status "unstable" .

# GRADUATE DEGREE
credType:graduateDegree a skos:Concept ;
  skos:prefLabel "Graduate Degree"@en-US ; 
  skos:definition "A graduate degree is a post-baccalaureate, advanced degree at the masters or professional level."@en-US ;
  skos:broader credType:degree ;
  skos:inScheme credType: ;
  vs:term_status "unstable" .
  
# DOCTORAL DEGREE
credType:doctoralDegree a skos:Concept ;
  skos:prefLabel "Doctoral Degree"@en-US ; 
  skos:definition "A doctorate degree is the highest level of academic degree."@en-US ;
  skos:broader credType:degree ;
  skos:inScheme credType: ;
  vs:term_status "unstable" .
  
# DIGITAL BADGE    
credType:digitalBadge a skos:Concept;
  skos:prefLabel "Digital Badge"@en-US; 
  skos:definition "Validated indicator of accomplishment, skill, quality, or interest that can be earned in many learning environments issued as a digital badge."@en-US;
  skos:inScheme credType: ;
  vs:term_status "unstable" .
  
# DIPLOMA   
credType:diploma a skos:Concept;
  skos:prefLabel "Diploma"@en-US; 
  skos:definition "Awarded by an educational establishment to show that someone has successfully completed a course of study or equivalent."@en-US;
  skos:inScheme credType: ;
  vs:term_status "unstable" .
  
# LICENSE   
credType:license a skos:Concept;
  skos:prefLabel "License"@en-US; 
  skos:definition "The permission granted by competent authority to exercise a certain privilege that, without such authorization, would constitute an illegal act."@en-US;
  skos:inScheme credType: ;
  vs:term_status "unstable" .
  
# MICRO-CREDENTIAL   
credType:microCredential a skos:Concept;
  skos:prefLabel "Micro-Credential"@en-US; 
  skos:definition "Validated indicator of accomplishment, skill, quality, or interest that can be earned in many learning environments such as MOOCs that may or may not be issued a digital badge."@en-US;
  skos:inScheme credType: ;
  vs:term_status "unstable" .
  
# MILITARY CREDENTIAL   
credType:militaryCredential a skos:Concept;
  skos:prefLabel "Military Credential"@en-US; 
  skos:definition "A qualification awarded by the military to show that a soldier is qualified to perform a job or task based on a course of study or equivalent experience."@en-US;
  skos:inScheme credType: ;
  vs:term_status "unstable" .
  
# NANODEGREE   
credType:nanodegree a skos:Concept;
  skos:prefLabel "Nanodegree"@en-US; 
  skos:definition "A nanodegree program is a compact online curriculum designed to get you the skills that employers believe are key to get a job in technology."@en-US;
  skos:scopeNote "A nonodegree focuses on learning by doing. It is typically comprised of 5 to 8 projects with relevant courses to support the skills needed to complete those projects."@en-US ;
  skos:inScheme credType: ;
  vs:term_status "unstable" .