@prefix credType: <https://w3id.org/ctdl/vocabs/credentialType/> .
@prefix dc: <http://purl.org/dc/elements/1.1/> .
@prefix dct: <http://purl.org/dc/terms/> .
@prefix skos: <http://www.w3.org/2004/02/skos/core#> .
@prefix schema: <http://schema.org/> .
@prefix rdf: <http://www.w3.org/1999/02/22-rdf-syntax-ns#> .
@prefix rdfs: <http://www.w3.org/2000/01/rdf-schema#> .
@prefix xsd: <http://www.w3.org/2001/XMLSchema#> .
@prefix adms: <http://www.w3.org/ns/adms#> .
@prefix bibo: <http://purl.org/ontology/bibo/status/> .
@prefix vs: <http://www.w3.org/2003/06/sw-vocab-status/ns#> .

credType: a skos:ConceptScheme;
   dc:title "CTI Credential Type Vocabulary" ;
   dc:creator "Credential Transparency Initiative (CTI)"@en-US ;
   dc:description "A concept scheme that defines the categories of credentials in the education-workforce development ecosystem."@en-US ;
   dct:created "2016-05-04"^^xsd:date ;
   dct:modified "2016-08-26"^^xsd:date ;
   skos:hasTopConcept credType:Apprenticeship ;
   skos:hasTopConcept credType:Badge ;
   skos:hasTopConcept credType:Certificate;
   skos:hasTopConcept credType:Certification;
   skos:hasTopConcept credType:Degree;  
   skos:hasTopConcept credType:Diploma;
   skos:hasTopConcept credType:License;
   skos:hasTopConcept credType:MicroCredential;
   skos:hasTopConcept credType:QualityAssuranceCredential;
   dct:source "Sources consulted include, but are not limited to: Integrated Postsecondary Education Data System (IPEDS) and Common Education Data Standards (CEDS)."@en-US ;
   dct:license <http://creativecommons.org/licenses/by/4.0/> ;                         
   adms:status bibo:draft . 
   
# BADGE
credType:Badge a skos:Concept;
  skos:prefLabel "Badge"@en-US; 
  skos:definition "A recognition designed to be displayed as a marker of accomplishment, activity, achievement, skill, interest, association, or identity."@en-US;
  skos:inScheme credType: ;
  vs:term_status "unstable" .
  
# DIGITAL BADGE
credType:DigitalBadge a skos:Concept;
  skos:prefLabel "Digital Badge"@en-US; 
  skos:definition "A badge offered in digital form."@en-US;
  skos:broader credType:Badge ;  
  skos:inScheme credType: ;
  vs:term_status "unstable" .
  
# OPEN BADGE
credType:OpenBadge a skos:Concept;
  skos:prefLabel "Open Badge"@en-US; 
  skos:definition "Visual symbols of accomplishments packed with verifiable learner data and evidence according to the Open Badges Specification."@en-US;
  skos:broader credType:Badge ; 
  skos:inScheme credType: ;
  vs:term_status "unstable" .  

# APPRENTICESHIP CERTIFICATE 
credType:apprenticeshipCertificate a skos:Concept ;
   skos:prefLabel "Apprenticeship Certificate"@en-US ; 
   skos:definition "A credential earned through work-based learning and postsecondary earn-and-learn models that meet national standards and are applicable to industry trades and professions."@en-US;
   skos:broader credType:certificate ;
   skos:inScheme credType: ;
   vs:term_status "unstable" .

# CERTIFICATE    
credType:certificate a skos:Concept;
  skos:prefLabel "Certificate"@en-US; 
  skos:definition "A credential that designates requisite mastery of the knowledge and skills of an occupation, profession, or academic program."@en-US;
  skos:narrower credType:apprenticeshipCertificate ;
  skos:inScheme credType: ;
  vs:term_status "unstable" .

# JOURNEYMAN CERTIFICATE  
credType:journeymanCertificate a skos:Concept;
  skos:prefLabel "Journeyman Certificate"@en-US; 
  skos:definition "A credential awarded to skilled workers on successful completion of an apprenticeship in industry trades and professions."@en-US;
  skos:broader credType:apprenticeshipCertificate;
  skos:inScheme credType: ;
  vs:term_status "unstable" .
  
# MASTER  CERTIFICATE  
credType:masterCertificate a skos:Concept;
  skos:prefLabel "Master Certificate"@en-US; 
  skos:definition "A credential awarded upon demonstration through apprenticeship of the the highest level of skills and performance in industry trades and professions."@en-US;
  skos:broader credType:apprenticeshipCertificate;
  skos:inScheme credType: ;
  vs:term_status "unstable" .
  
# CERTIFICATION    
credType:certification a skos:Concept;
  skos:prefLabel "Certification"@en-US; 
  skos:definition "A time-limited, renewable non-degree credential awarded by an authoritative body to an individual or organization for demonstrating the designated knowledge, skills, and abilities to perform a specific job."@en-US;
  skos:inScheme credType: ;
  vs:term_status "unstable" . 
  
# DEGREE    
credType:degree a skos:Concept ;
  skos:prefLabel "Degree"@en-US ; 
  skos:definition "An academic credential conferred upon completion of a program or course of study, typically over multiple years at postsecondary education institutions."@en-US ;
  skos:narrower credType:associateDegree ; 
  skos:narrower credType:bachelorDegree ;
  skos:narrower credType:masterDegree ; 
  skos:narrower credType:doctoralDegree ;    
  skos:inScheme credType: ;
  vs:term_status "unstable" .
  
# ASSOCIATE DEGREE
credType:associateDegree a skos:Concept ;
  skos:prefLabel "Associate Degree"@en-US ; 
  skos:definition "An award level that normally requires at least 2 but less than 4 years of full-time equivalent college-level work."@en-US ;
  skos:broader credType:degree ;
  skos:inScheme credType: ;
  vs:term_status "unstable" .
  
# BACHELOR'S DEGREE
credType:bachelorDegree a skos:Concept ;
  skos:prefLabel "Bachelor's Degree"@en-US ; 
  skos:definition "An award level that normally requires at least 4 but not more than 5 years of full-time equivalent college-level work."@en-US ;
  skos:broader credType:degree ;
  skos:inScheme credType: ;
  vs:term_status "unstable" .

# MASTER'S DEGREE
credType:masterDegree a skos:Concept ;
  skos:prefLabel "Master's Degree"@en-US ; 
  skos:definition "An award level that requires the successful completion of a program of study of at least the full-time equivalent of 1 but not more than 2 academic years of work beyond the bachelor's degree."@en-US ;
  skos:broader credType:degree ;
  skos:inScheme credType: ;
  vs:term_status "unstable" .
  
# DOCTORAL DEGREE
credType:doctoralDegree a skos:Concept ;
  skos:prefLabel "Doctoral Degree"@en-US ; 
  skos:definition "The highest award level to be earned for postsecondary study."@en-US ;
  skos:broader credType:degree ;
  skos:narrower credType:researchDoctorate ;
  skos:narrower credType:professionalDoctorate ;     
  skos:inScheme credType: ;
  vs:term_status "unstable" .
  
# RESEARCH DOCTORATE
credType:researchDoctorate a skos:Concept ;
  skos:prefLabel "Research Doctorate"@en-US ; 
  skos:definition "A doctoral degree conferred for advanced work beyond the master level, including the preparation and defense of a thesis or dissertation based on original research, or the planning and execution of an original project demonstrating substantial artistic or scholarly achievement."@en-US ;
  skos:broader credType:doctoralDegree ;
  skos:inScheme credType: ;
  vs:term_status "unstable" .
  
# PROFESSIONAL DOCTORATE
credType:professionalDoctorate a skos:Concept ;
  skos:prefLabel "Professional Doctorate"@en-US ; 
  skos:definition "A doctoral degree conferred upon completion of a program providing the knowledge and skills for the recognition, credential, or license required for professional practice."@en-US ;
  skos:broader credType:doctoralDegree ;
  skos:inScheme credType: ;
  vs:term_status "unstable" .  
  
# DIPLOMA   
credType:diploma a skos:Concept;
  skos:prefLabel "Diploma"@en-US; 
  skos:definition "Awarded by an educational establishment to show that someone has successfully completed a course of study or equivalent."@en-US;
  skos:narrower credType:secondarySchoolDiploma ;
  skos:narrower credType:generalEducationDevelopment ;  
  skos:inScheme credType: ;
  vs:term_status "unstable" .
  
# SECONDARY SCHOOL DIPLOMA
credType:secondarySchoolDiploma a skos:Concept;
  skos:prefLabel "Secondary School Diploma"@en-US; 
  skos:definition "A diploma awarded by secondary education institutions for successful completion of a secondary school program typically lasting four years."@en-US;
  skos:broader credType:diploma ;
  skos:inScheme credType: ;
  vs:term_status "unstable" .

# GENERAL EDUCATION DEVELOPMENT (GED)
credType:generalEducationDevelopment a skos:Concept;
  skos:prefLabel "General Education Development (GED)"@en-US; 
  skos:definition "A credential awarded by examination that demonstrates that an individual has acquired secondary school-level academic skills."@en-US;
  skos:broader credType:diploma ;
  skos:inScheme credType: ;
  vs:term_status "unstable" .

# LICENSE   
credType:license a skos:Concept;
  skos:prefLabel "License"@en-US; 
  skos:definition "A credential awarded by a government agency that constitutes legal authority to do a specific job and/or utilize a specific item, system or infrastructure and are typically earned through some combination of degree or certificate attainment, certifications, assessments, work experience, and/or fees, and are time-limited and must be renewed periodically."@en-US;
  skos:inScheme credType: ;
  vs:term_status "unstable" .
  
# MICRO-CREDENTIAL   
credType:microCredential a skos:Concept;
  skos:prefLabel "Micro-Credential"@en-US; 
  skos:definition "A credential that attests to achievement of a specific knowledge, skill, or competency."@en-US;
  skos:inScheme credType: ;
  vs:term_status "unstable" .
  
# QUALITY ASSURANCE CREDENTIAL   
credType:qualityAssuranceCredential a skos:Concept;
  skos:prefLabel "Quality Assurance Credential"@en-US; 
  skos:definition "A credential assuring that an organization, program, or awarded credential meets prescribed requirements and may include development and administration of qualifying examinations."@en-US;
  skos:inScheme credType: ;
  vs:term_status "unstable" .