@prefix inputType: <https://purl.org/ctdl/vocabs/inputType/> .
@prefix dc: <http://purl.org/dc/elements/1.1/> .
@prefix dct: <http://purl.org/dc/terms/> .
@prefix skos: <http://www.w3.org/2004/02/skos/core#> .
@prefix schema: <http://schema.org/> .
@prefix rdf: <http://www.w3.org/1999/02/22-rdf-syntax-ns#> .
@prefix rdfs: <http://www.w3.org/2000/01/rdf-schema#> .
@prefix xsd: <http://www.w3.org/2001/XMLSchema#> .
@prefix adms: <http://www.w3.org/ns/adms#> .
@prefix bibo: <http://purl.org/ontology/bibo/status/> .
@prefix vs: <http://www.w3.org/2003/06/sw-vocab-status/ns#> .

# EXTERNAL INPUT TYPE VOCABULARY DESCRIPTION
inputType: a skos:ConceptScheme;
    dc:title "CTI Cost Type Vocabulary" ;
    dc:creator "Credential Transparency Initiative (CTI)"@en-US ;
    dc:description "A concept scheme that defines the types of external input engaged in a process."@en-US ;
    dct:created "2016-09-08"^^xsd:date ;
    dct:license <http://creativecommons.org/licenses/by/4.0/> ;                         
    adms:status bibo:draft . 
   
# CONCEPT: CONSUMERS
inputType:Consumers a skos:Concept;
    skos:prefLabel "Consumers"@en-US; 
    skos:definition "External stakeholder review, guidance or recommendations by consumers."@en-US;
    skos:inScheme inputType: ;
    vs:term_status "unstable" .
    
# CONCEPT: EDUCATION ADMINISTRATORS
inputType:EducationAdministrators a skos:Concept;
    skos:prefLabel "@@@"@en-US; 
    skos:definition "External stakeholder review, guidance or recommendations by education administrators."@en-US;
    skos:inScheme inputType: ;
    vs:term_status "unstable" .    
       
# CONCEPT: FACULTY
inputType:Faculty a skos:Concept;
    skos:prefLabel "Faculty"@en-US; 
    skos:definition "External stakeholder review, guidance or recommendations by faculty."@en-US;
    skos:inScheme inputType: ;
    vs:term_status "unstable" .
    
# CONCEPT: STUDENTS
inputType:Students a skos:Concept;
    skos:prefLabel "Students"@en-US; 
    skos:definition "External stakeholder review, guidance or recommendations by students."@en-US;
    skos:inScheme inputType: ;
    vs:term_status "unstable" .
       
# CONCEPT: NATIONAL GOVERNMENT
inputType:NationalGovernment a skos:Concept;
    skos:prefLabel "Federal/National Government"@en-US; 
    skos:definition "External stakeholder review, guidance or recommendations by federal or national government."@en-US;
    skos:inScheme inputType: ;
    vs:term_status "unstable" .
    
# CONCEPT: INDUSTRY EMPLOYERS
inputType:IndustryEmployers a skos:Concept;
    skos:prefLabel "Industry Employers"@en-US; 
    skos:definition "External stakeholder review, guidance or recommendations by industry employers."@en-US;
    skos:inScheme inputType: ;
    vs:term_status "unstable" .
       
# CONCEPT: INDUSTRY PRACTIONERS
inputType:IndustryPractitioners a skos:Concept;
    skos:prefLabel "Industry Practitioners"@en-US; 
    skos:definition "External stakeholder review, guidance or recommendations by industry practitioners."@en-US;
    skos:inScheme inputType: ;
    vs:term_status "unstable" .
    
# CONCEPT: ASSOCIATIONS
inputType:Associations a skos:Concept;
    skos:prefLabel "Industry Professional Associations"@en-US; 
    skos:definition "External stakeholder review, guidance or recommendations by industry professional associations."@en-US;
    skos:inScheme inputType: ;
    vs:term_status "unstable" .  
       
# CONCEPT: EXPERTS
inputType:Experts a skos:Concept;
    skos:prefLabel "Industry Subject Matter Experts"@en-US; 
    skos:definition "External stakeholder review, guidance or recommendations by industry subject matter experts."@en-US;
    skos:inScheme inputType: ;
    vs:term_status "unstable" .
    
# CONCEPT: LOCAL GOVERNMENT
inputType:LocalGovernment a skos:Concept;
    skos:prefLabel "Local Government"@en-US; 
    skos:definition "External stakeholder review, guidance or recommendations by local government."@en-US;
    skos:inScheme inputType: ;
    vs:term_status "unstable" .   
       
# CONCEPT: STATE/PROVINCIAL GOVERNMENT
inputType:StateGovernment a skos:Concept;
    skos:prefLabel "State/Provincial Government"@en-US; 
    skos:definition "External stakeholder review, guidance or recommendations by state or provincial government."@en-US;
    skos:inScheme inputType: ;
    vs:term_status "unstable" .
    
# CONCEPT: INTERNATIONAL BODIES
inputType:InternationalBodies a skos:Concept;
    skos:prefLabel "International Bodies"@en-US; 
    skos:definition "External stakeholder review, guidance or recommendations by international bodies."@en-US;
    skos:inScheme inputType: ;
    vs:term_status "unstable" .       