@prefix intendedPurpose: <https://purl.org/ctdl/vocabs/intendedPurpose/> .
@prefix dc: <http://purl.org/dc/elements/1.1/> .
@prefix dct: <http://purl.org/dc/terms/> .
@prefix skos: <http://www.w3.org/2004/02/skos/core#> .
@prefix schema: <http://schema.org/> .
@prefix rdf: <http://www.w3.org/1999/02/22-rdf-syntax-ns#> .
@prefix rdfs: <http://www.w3.org/2000/01/rdf-schema#> .
@prefix xsd: <http://www.w3.org/2001/XMLSchema#> .
@prefix adms: <http://www.w3.org/ns/adms#> .
@prefix bibo: <http://purl.org/ontology/bibo/status/> .
@prefix vs: <http://www.w3.org/2003/06/sw-vocab-status/ns#> .

# INTENDED PURPOSE VOCABULARY DESCRIPTION
intendedPurpose: a skos:ConceptScheme;
    dc:title "CTI Intended Purpose Vocabulary" ;
    dc:creator "Credential Transparency Initiative (CTI)"@en-US ;
    dc:description "A concept scheme describing the intended types of application of the credential by the holder."@en-US ;
    dct:created "2016-09-07"^^xsd:date ;
    dct:license <http://creativecommons.org/licenses/by/4.0/> ;                         
    adms:status bibo:draft . 
   
# CONCEPT: GENERAL EDUCATION
intendedPurpose:GeneralEducation a skos:Concept;
    skos:prefLabel "GeneralEducation"@en-US; 
    skos:definition "The holder's intended purpose in earning the credential is for general education."@en-US;
    skos:inScheme intendedPurpose: ;
    vs:term_status "unstable" .
       
# CONCEPT: JOB OR CAREER PREPARATION
intendedPurpose:JobOrCareerPreparation a skos:Concept;
    skos:prefLabel "Job/CareerPreparation"@en-US; 
    skos:definition "The holder's intended purpose in earning the credential is for job or career preparation."@en-US;
    skos:inScheme intendedPurpose: ;
    vs:term_status "unstable" .
       
# CONCEPT: PRIOR LEARNING EXPERIENCE
intendedPurpose:priorExperience a skos:Concept;
    skos:prefLabel "Prior Learning Experience"@en-US; 
    skos:definition "The holder's intended purpose in earning the credential is for prior learning experience."@en-US;
    skos:inScheme intendedPurpose: ;
    vs:term_status "unstable" .
       
# CONCEPT: MID-CAREER LEVEL ADVANCEMENT (???)
intendedPurpose:MidCareer a skos:Concept;
    skos:prefLabel "Mid-Career Level"@en-US; 
    skos:definition "The holder's intended purpose in earning the credential is for mid-career level (advancement?)."@en-US;
    skos:inScheme intendedPurpose: ;
    vs:term_status "unstable" .