@prefix learnSchedule: <https://purl.org/ctdl/vocabs/learningSchedule/> .
@prefix dc: <http://purl.org/dc/elements/1.1/> .
@prefix dct: <http://purl.org/dc/terms/> .
@prefix skos: <http://www.w3.org/2004/02/skos/core#> .
@prefix schema: <http://schema.org/> .
@prefix rdf: <http://www.w3.org/1999/02/22-rdf-syntax-ns#> .
@prefix rdfs: <http://www.w3.org/2000/01/rdf-schema#> .
@prefix xsd: <http://www.w3.org/2001/XMLSchema#> .
@prefix adms: <http://www.w3.org/ns/adms#> .
@prefix bibo: <http://purl.org/ontology/bibo/status/> .
@prefix vs: <http://www.w3.org/2003/06/sw-vocab-status/ns#> .

# LEARNING SCHEDULE TYPE VOCABULARY DESCRIPTION
learnSchedule: a skos:ConceptScheme;
    dc:title "CTI Learning Schedule Vocabulary" ;
    dc:creator "Credential Transparency Initiative (CTI)"@en-US ;
    dc:description "A concept scheme that defines the types of learning schedule."@en-US ;
    dct:created "2016-09-08"^^xsd:date ;
    dct:modified "2016-09-30"^^xsd:date ;    
    dct:license <http://creativecommons.org/licenses/by/4.0/> .                         
   
# CONCEPT: FULL-TIME
learnSchedule:FullTime a skos:Concept;
    skos:prefLabel "Full-Time"@en-US; 
    skos:definition "A full-time learning schedule supports a focus on academic and skills development that is intensive and without interruption."@en-US;
    skos:inScheme learnSchedule: .
   
# CONCEPT: PART-TIME
learnSchedule:PartTime a skos:Concept;
    skos:prefLabel "Part-Time"@en-US; 
    skos:definition "A part-time learning schedule supports academic and skills development that is less than full-time and shares focus with other activities such as work and family commitments."@en-US;
    skos:inScheme learnSchedule: .
       
# CONCEPT: SELF-PACED
learnSchedule:SelfPaced@ a skos:Concept;
    skos:prefLabel "Self-Paced@"@en-US; 
    skos:definition "A self-paced learning schedule supports academic and skills development based on the needs of individual learner."@en-US;
    skos:inScheme learnSchedule: .
