@prefix learnDelivery: <https://purl.org/ctdl/vocabs/learningDelivery/> .
@prefix dc: <http://purl.org/dc/elements/1.1/> .
@prefix dct: <http://purl.org/dc/terms/> .
@prefix skos: <http://www.w3.org/2004/02/skos/core#> .
@prefix schema: <http://schema.org/> .
@prefix rdf: <http://www.w3.org/1999/02/22-rdf-syntax-ns#> .
@prefix rdfs: <http://www.w3.org/2000/01/rdf-schema#> .
@prefix xsd: <http://www.w3.org/2001/XMLSchema#> .
@prefix adms: <http://www.w3.org/ns/adms#> .
@prefix bibo: <http://purl.org/ontology/bibo/status/> .
@prefix vs: <http://www.w3.org/2003/06/sw-vocab-status/ns#> .

# LEARNING DELIVERY TYPE VOCABULARY DESCRIPTION
learnDelivery: a skos:ConceptScheme;
    dc:title "CTI Cost Type Vocabulary" ;
    dc:creator "Credential Transparency Initiative (CTI)"@en-US ;
    dc:description "A concept scheme that defines the types of learning delivery."@en-US ;
    dct:created "2016-09-08"^^xsd:date ;
    dct:license <http://creativecommons.org/licenses/by/4.0/> ;                         
    adms:status bibo:draft . 
   
# CONCEPT: BLENDED LEARNING
learnDelivery:BlendedLearning a skos:Concept;
    skos:prefLabel "Blended Learning"@en-US; 
    skos:definition "Instructional activity in which a student learns through a combination of content delivery through digital and online media and through face-to-face or technology supported synchronous interactions among students and instructor."@en-US;
    skos:inScheme learnDelivery: ;
    vs:term_status "unstable" .
    
# CONCEPT: BROADCAST
learnDelivery:Broadcast a skos:Concept;
    skos:prefLabel "Broadcast"@en-US; 
    skos:definition "Technology-mediated learning based on simultaneous, one-way communication of instructional content from the instructor to the learners."@en-US;
    skos:inScheme learnDelivery: ;
    vs:term_status "unstable" .
    
# CONCEPT: COMPETENCY BASED
learnDelivery:CompetencyBased a skos:Concept;
    skos:prefLabel "Competency Based"@en-US; 
    skos:definition "Progress through a learning opportunity, task or assessment based on the attainment of competencies."@en-US;
    skos:inScheme learnDelivery: ;
    vs:term_status "unstable" .        
       
# CONCEPT: CORRESPONDENCE
learnDelivery:Correspondence a skos:Concept;
    skos:prefLabel "Correspondence"@en-US; 
    skos:definition "Learning based primarily on asynchronous, written communications between learner and instructor using conventional postal mechanisms."@en-US;
    skos:inScheme learnDelivery: ;
    vs:term_status "unstable" .
    
# CONCEPT: EARLY COLLEGE
learnDelivery:EarlyCollege a skos:Concept;
    skos:prefLabel "Early College"@en-US; 
    skos:definition "[TBD]"@en-US;
    skos:inScheme learnDelivery: ;
    vs:term_status "unstable" .
    
# CONCEPT: FACE TO FEACE
learnDelivery:FaceToFace a skos:Concept;
    skos:prefLabel "Face to Face"@en-US; 
    skos:definition "Learning that takes place with instructor and learners in each other's presence."@en-US;
    skos:inScheme learnDelivery: ;
    vs:term_status "unstable" .
       
# CONCEPT: INDEPENDENT STUDY
learnDelivery:IndependentStudy a skos:Concept;
    skos:prefLabel "Independent Study"@en-US; 
    skos:definition "A learning activity that is undertaken by an individual with little to no supervision."@en-US;
    skos:inScheme learnDelivery: ;
    vs:term_status "unstable" .
    
# CONCEPT: INTERACTIVE MEDIA
learnDelivery:InteractiveMedia a skos:Concept;
    skos:prefLabel "Interactive Audio/Video"@en-US; 
    skos:definition "A learning activity in which a computer-based system responds to the learner's actions by presenting content through various forms of media (e.g., moving image, animation, video, audio, and video games)."@en-US;
    skos:inScheme learnDelivery: ;
    vs:term_status "unstable" .
    
# CONCEPT: ONLINE
learnDelivery:Online a skos:Concept;
    skos:prefLabel "Online"@en-US; 
    skos:definition "A computer network mediated learning experience."@en-US;
    skos:inScheme learnDelivery: ;
    vs:term_status "unstable" .