@prefix skos: <http://www.w3.org/2004/02/skos/core#> .
@prefix dct: <http://purl.org/dc/terms/> .
@prefix omr: <http://metadataregistry.org/uri/> .

<http://connectingcredentials.org/vocabs/levels/> a skos:ConceptScheme ;
  dct:title "Connecting Credentials Levels"@en-US ;
  dct:description "The level requirements and competencies in study and work are described in terms of the degree of adaptability, complexity, range and selectivity."@en-US ;
  skos:hasTopConcept [<http://connectingcredentials.org/vocabs/levels/level1>,
    <http://connectingcredentials.org/vocabs/levels/level2>,
    <http://connectingcredentials.org/vocabs/levels/level3>,
    <http://connectingcredentials.org/vocabs/levels/level4>,
    <http://connectingcredentials.org/vocabs/levels/level5>,
    <http://connectingcredentials.org/vocabs/levels/level6>,
    <http://connectingcredentials.org/vocabs/levels/level7>,
    <http://connectingcredentials.org/vocabs/levels/level8>]

<http://connectingcredentials.org/vocabs/levels/level1> a skos:Concept ;
  skos:prefLabel "Level 1"@en-US ;
  skos:definition "Demonstrates achievement of fundamental competencies to complete narrow and limited tasks within a highly structured field of study or work under direct supervision or guidance."@en-US ;
  skos:inScheme <http://connectingcredentials.org/vocabs/levels/> ;
  skos:isTopConceptOf <http://connectingcredentials.org/vocabs/levels/> .

<http://connectingcredentials.org/vocabs/levels/level2> a skos:Concept ;
  skos:prefLabel "Level 2"@en-US ;
  skos:definition "Demonstrates achievement of fundamental competencies to complete technical, routine tasks within a structured field of study or work largely subject to overall direction or guidance."@en-US ;
  skos:inScheme <http://connectingcredentials.org/vocabs/levels/> ;
  skos:isTopConceptOf <http://connectingcredentials.org/vocabs/levels/> .

<http://connectingcredentials.org/vocabs/levels/level3> a skos:Concept ;
  skos:prefLabel "Level 3"@en-US ;
  skos:definition "Demonstrates competencies for processing well-defined technical tasks that are less structured and include non-routine tasks. These tasks have some degree of complexity, assigned within a comprehensive field of study or occupational activity subject to some change and largely subject to overall supervision or guidance."@en-US ;
  skos:inScheme <http://connectingcredentials.org/vocabs/levels/> ;
  skos:isTopConceptOf <http://connectingcredentials.org/vocabs/levels/> .

<http://connectingcredentials.org/vocabs/levels/level4> a skos:Concept ;
  skos:prefLabel "Level 4"@en-US ;
  skos:definition "Demonstrates competencies for the processing of specialized and complex tasks within a comprehensive field of study or an occupational environment that is subject to change. This requires theoretical knowledge and practical skills to select appropriate principles and procedures and may involve overall supervision."@en-US ;
  skos:inScheme <http://connectingcredentials.org/vocabs/levels/> ;
  skos:isTopConceptOf <http://connectingcredentials.org/vocabs/levels/> .  

<http://connectingcredentials.org/vocabs/levels/level5> a skos:Concept ;
  skos:prefLabel "Level 5"@en-US ;
  skos:definition "Demonstrates advanced competencies for the processing of comprehensive tasks assigned within a complex and specialized field of study or occupational activity subject to change. This requires the ability to select and apply appropriate theoretical knowledge and practical skills to perform technical tasks in a broad range of contexts"@en-US ;
  skos:inScheme <http://connectingcredentials.org/vocabs/levels/> ;
  skos:isTopConceptOf <http://connectingcredentials.org/vocabs/levels/> .

<http://connectingcredentials.org/vocabs/levels/level6> a skos:Concept ;
  skos:prefLabel "Level 6"@en-US ;
  skos:definition "Demonstrates mastery in the processing of comprehensive tasks and problems within subareas of a field of study or within a field of occupational activity characterized by a high degree of complexity and by frequent changes. This requires a high degree of theoretical knowledge and practical skills."@en-US ;
  skos:inScheme <http://connectingcredentials.org/vocabs/levels/> ;
  skos:isTopConceptOf <http://connectingcredentials.org/vocabs/levels/> .

<http://connectingcredentials.org/vocabs/levels/level7> a skos:Concept ;
  skos:prefLabel "Level 7"@en-US ;
  skos:definition "Demonstrates competencies for the processing of new and complex professional tasks and problem settings within a scientific subject or an occupational field characterized by frequent and unpredictable changes. This requires the need to elucidate the major theories and the application of advanced specialized knowledge, research methods and approaches in various contexts."@en-US ;
  skos:inScheme <http://connectingcredentials.org/vocabs/levels/> ;
  skos:isTopConceptOf <http://connectingcredentials.org/vocabs/levels/> .

<http://connectingcredentials.org/vocabs/levels/level8> a skos:Concept ;
  skos:prefLabel "Level 8"@en-US ;
  skos:definition "Demonstrates competencies for obtaining research findings in a scientific subject or for the development of innovative solutions and procedures in highly complex and novel problem situations within a field of occupational activity. This requires a capacity for a wide range of strategic and scientific thinking and creative action."@en-US ;
  skos:inScheme <http://connectingcredentials.org/vocabs/levels/> ;
  skos:isTopConceptOf <http://connectingcredentials.org/vocabs/levels/> .