@prefix audLevel: <https://purl.org/ctdl/vocabs/audienceLevel/> .
@prefix dc: <http://purl.org/dc/elements/1.1/> .
@prefix dct: <http://purl.org/dc/terms/> .
@prefix skos: <http://www.w3.org/2004/02/skos/core#> .
@prefix schema: <http://schema.org/> .
@prefix rdf: <http://www.w3.org/1999/02/22-rdf-syntax-ns#> .
@prefix rdfs: <http://www.w3.org/2000/01/rdf-schema#> .
@prefix xsd: <http://www.w3.org/2001/XMLSchema#> .
@prefix adms: <http://www.w3.org/ns/adms#> .
@prefix bibo: <http://purl.org/ontology/bibo/status/> .
@prefix vs: <http://www.w3.org/2003/06/sw-vocab-status/ns#> .

# AUDIENCE LEVEL VOCABULARY DESCRIPTION
audLevel: a skos:ConceptScheme;
    dc:title "CTI Audience Level Vocabulary" ;
    dc:creator "Credential Transparency Initiative (CTI)"@en-US ;
    dc:description "A concept scheme that defines the levels of the audience for a resource."@en-US ;
    dct:created "2016-09-07"^^xsd:date ;
    dct:license <http://creativecommons.org/licenses/by/4.0/> ;                         
    adms:status bibo:draft . 
   
# CONCEPT: ELEMENTARY SCHOOL
audLevel:ElementarySchool a skos:Concept;
    skos:prefLabel "Elementary School"@en-US; 
    skos:definition "A school for students in their first school years, before they enter secondary education."@en-US;
    skos:inScheme audLevel: ;
    vs:term_status "unstable" .

# CONCEPT: KINDERGARTEN
audLevel:Kindergarten a skos:Concept;
    skos:prefLabel "Kindergarten"@en-US; 
    skos:definition "A school or class that prepares children for the first year of elementary school education."@en-US;
    skos:inScheme audLevel: ;
    vs:term_status "unstable" .

# CONCEPT: MIDDLE SCHOOL
audLevel:MiddleSchool a skos:Concept;
    skos:prefLabel "Middle School"@en-US; 
    skos:definition "A intermediate school between an elementary school and a high school."@en-US;
    skos:inScheme audLevel: ;
    vs:term_status "unstable" .

# CONCEPT: POSTSECONDARY 1-3
audLevel:Postsecondary1-3 a skos:Concept;
    skos:prefLabel "Postsecondary (1-3 years)"@en-US; 
    skos:definition "A post-secondary level between the 1st year and the 3rd year."@en-US;
    skos:inScheme audLevel: ;
    vs:term_status "unstable" .
    
# CONCEPT: POSTSECONDARY 3-6
audLevel:Postsecondary3-6 a skos:Concept;
    skos:prefLabel "Postsecondary (3-6 years)"@en-US; 
    skos:definition "A post-secondary level between the 3rd year and the 6th year."@en-US;
    skos:inScheme audLevel: ;
    vs:term_status "unstable" .
    
# CONCEPT: POSTSECONDARY 6 AND OVER
audLevel:Postsecondary6andOver a skos:Concept;
    skos:prefLabel "Postsecondary (6+ years)"@en-US; 
    skos:definition "A post-secondary level from the 6th year and beyond."@en-US;
    skos:inScheme audLevel: ;
    vs:term_status "unstable" .
    
# CONCEPT: POSTSECONDARY 6 AND OVER
audLevel:PostsecondaryUnder1 a skos:Concept;
    skos:prefLabel "Postsecondary (Less than 1 year)"@en-US; 
    skos:definition "A post-secondary level under 1 year."@en-US;
    skos:inScheme audLevel: ;
    vs:term_status "unstable" .
    
# CONCEPT: SECONDARY SCHOOL
audLevel:SecondarySchool a skos:Concept ;
    skos:prefLabel "Secondary School"@en-US ; 
    skos:definition "A school that typically comprises year 9 through year 12 of study."@en-US ;
    skos:inScheme audLevel: ;
    vs:term_status "unstable" .
    
# CONCEPT: TECHNICAL SCHOOL
audLevel:TechnicalSchool a skos:Concept ;
    skos:prefLabel "Technical School"@en-US ; 
    skos:definition "A general term used for a two-year, post-secondary college. "@en-US ;
    skos:inScheme audLevel: ;
    vs:term_status "unstable" .                                    