@prefix claimType: <https://purl.org/ctdl/vocabs/claimType/> .
@prefix dc: <http://purl.org/dc/elements/1.1/> .
@prefix dct: <http://purl.org/dc/terms/> .
@prefix skos: <http://www.w3.org/2004/02/skos/core#> .
@prefix schema: <http://schema.org/> .
@prefix rdf: <http://www.w3.org/1999/02/22-rdf-syntax-ns#> .
@prefix rdfs: <http://www.w3.org/2000/01/rdf-schema#> .
@prefix xsd: <http://www.w3.org/2001/XMLSchema#> .
@prefix adms: <http://www.w3.org/ns/adms#> .
@prefix bibo: <http://purl.org/ontology/bibo/status/> .
@prefix vs: <http://www.w3.org/2003/06/sw-vocab-status/ns#> .

# COST TYPE VOCABULARY DESCRIPTION
claimType: a skos:ConceptScheme;
    dc:title "CTI Claim Type Vocabulary" ;
    dc:creator "Credential Transparency Initiative (CTI)"@en-US ;
    dc:description "A concept scheme that defines the types of claims made."@en-US ;
    dct:created "2016-09-07"^^xsd:date ;
    dct:license <http://creativecommons.org/licenses/by/4.0/> ;                         
    adms:status bibo:draft . 
   
# CONCEPT: VERIFIED CLAIM
claimType:VerifiedClaim a skos:Concept;
    skos:prefLabel "Verified Claim"@en-US; 
    skos:definition "Verifiable representation of the credential holder's credential that is controlled by the credentialing organization."@en-US;
    skos:inScheme claimType: ;
    vs:term_status "unstable" .
    
# CONCEPT: BADGE CLAIM
claimType:BadgeClaim a skos:Concept;
    skos:prefLabel "Badge Claim"@en-US; 
    skos:definition "Verifiable representation of a credential holderâ€™s badge that is controlled by the credentialing organization."@en-US;
    skos:inScheme claimType: ;
    vs:term_status "unstable" .

# CONCEPT: TRANSCRIPT CLAIM
claimType:TranscriptClaim a skos:Concept;
    skos:prefLabel "Transcript Claim"@en-US; 
    skos:definition "Verifiable representation of postsecondary courses and degrees that is controlled by the credentialing organization."@en-US;
    skos:inScheme claimType: ;
    vs:term_status "unstable" .   