@prefix costType: <https://purl.org/ctdl/vocabs/costType/> .
@prefix dc: <http://purl.org/dc/elements/1.1/> .
@prefix dct: <http://purl.org/dc/terms/> .
@prefix skos: <http://www.w3.org/2004/02/skos/core#> .
@prefix schema: <http://schema.org/> .
@prefix rdf: <http://www.w3.org/1999/02/22-rdf-syntax-ns#> .
@prefix rdfs: <http://www.w3.org/2000/01/rdf-schema#> .
@prefix xsd: <http://www.w3.org/2001/XMLSchema#> .
@prefix adms: <http://www.w3.org/ns/adms#> .
@prefix vs: <http://www.w3.org/2003/06/sw-vocab-status/ns#> .

# COST TYPE VOCABULARY DESCRIPTION
costType: a skos:ConceptScheme;
    dc:title "CTI Cost Type Vocabulary" ;
    dc:creator "Credential Transparency Initiative (CTI)"@en-US ;
    dc:description "A concept scheme that defines the types of costs of a resource."@en-US ;
    dct:created "2016-09-07"^^xsd:date ;
    dct:modified "2016-09-28"^^xsd:date ;
    dct:license <http://creativecommons.org/licenses/by/4.0/> .                         
   
# CONCEPT: AGGREGATE COST
costType:AggregateCost a skos:Concept;
    skos:prefLabel "Aggregate Cost"@en-US; 
    skos:definition "The sum of direct costs."@en-US;
    skos:inScheme costType: .

# CONCEPT: APPLICATION
costType:Application a skos:Concept;
    skos:prefLabel "Application"@en-US; 
    skos:definition "Direct cost of applying for a learning opportunity (including programs of study), credential, assessment, or required task."@en-US;
    skos:inScheme costType: .
    
# CONCEPT: BACKGROUND CHECK
costType:BackgroundCheck a skos:Concept;
    skos:prefLabel "Background Check"@en-US; 
    skos:definition "Direct cost for performance of a required backgroung check."@en-US;
    skos:inScheme costType: . 
   
# CONCEPT: LEARNING RESOURCE
costType:LearningResource a skos:Concept;
    skos:prefLabel "Learning Resource"@en-US; 
    skos:definition "Direct costs for learning resources such as textbooks, workbooks, labratory fees, and related supplies."@en-US;
    skos:inScheme costType: .
    
# CONCEPT: STANDALONE/EXTRA ASSESSMENT
costType:StandaloneAssessment a skos:Concept;
    skos:prefLabel "Standalone/Extra Assessment"@en-US; 
    skos:definition "Direct costs of assessments not included as part of a learning opportunity,"@en-US;
    skos:inScheme costType: . 
   
# CONCEPT: TUITION
costType:Tuition a skos:Concept;
    skos:prefLabel "Tuition"@en-US; 
    skos:definition "Direct costs charged for teaching or instruction by a school, college, or university."@en-US;
    skos:inScheme costType: .
          