@prefix residency: <https://purl.org/ctdl/vocabs/residency/> .
@prefix dc: <http://purl.org/dc/elements/1.1/> .
@prefix dct: <http://purl.org/dc/terms/> .
@prefix skos: <http://www.w3.org/2004/02/skos/core#> .
@prefix schema: <http://schema.org/> .
@prefix rdf: <http://www.w3.org/1999/02/22-rdf-syntax-ns#> .
@prefix rdfs: <http://www.w3.org/2000/01/rdf-schema#> .
@prefix xsd: <http://www.w3.org/2001/XMLSchema#> .
@prefix adms: <http://www.w3.org/ns/adms#> .
@prefix bibo: <http://purl.org/ontology/bibo/status/> .
@prefix vs: <http://www.w3.org/2003/06/sw-vocab-status/ns#> .

# RESIDENCY TYPE TYPE VOCABULARY DESCRIPTION
residency: a skos:ConceptScheme;
    dc:title "CTI Cost Type Vocabulary" ;
    dc:creator "Credential Transparency Initiative (CTI)"@en-US ;
    dc:description "A concept scheme that defines the types of legal residency or domicile of learners."@en-US ;
    dct:created "2016-09-08"^^xsd:date ;
    dct:license <http://creativecommons.org/licenses/by/4.0/> ;                         
    adms:status bibo:draft . 
   
# CONCEPT: IN-STATE
residency:InState a skos:Concept;
    skos:prefLabel "In-State"@en-US; 
    skos:definition "The legal residency or domicile status of the agent is the state or province of the relevant activity."@en-US;
    skos:inScheme residency: ;
    vs:term_status "unstable" .
       
# CONCEPT: INTERNATIONAL
residency:International a skos:Concept;
    skos:prefLabel "International"@en-US; 
    skos:definition "The legal residency, domicile, or citizen status of the agent is the foreign nation."@en-US;
    skos:inScheme residency: ;
    vs:term_status "unstable" .
       
# CONCEPT: LOCAL
residency:Local a skos:Concept;
    skos:prefLabel "Local"@en-US; 
    skos:definition "The legal residency or domicile status of the agent is local."@en-US;
    skos:inScheme residency: ;
    vs:term_status "unstable" .
       
# CONCEPT: OUT-OF-STATE
residency:OutOfState a skos:Concept;
    skos:prefLabel "Out-of-State"@en-US; 
    skos:definition "The legal residency or domicile status of the agent is a state or province different from the state or provincial locus of the relevant activity."@en-US;
    skos:inScheme residency: ;
    vs:term_status "unstable" .
       
# CONCEPT: REGIONAL
residency:Regional a skos:Concept;
    skos:prefLabel "Regional"@en-US; 
    skos:definition "The legal residency or domicile status of the agent is the same geopolitical region as that of the relevant activity."@en-US;
    skos:inScheme residency: ;
    vs:term_status "unstable" .